Spec exponent

code/experimental/P256/Hacl.Spec.ECDSA.fst
@@ -1,7 +1,7 @@
 module Hacl.Spec.ECDSA
 
 open FStar.Mul 
-open Hacl.Spec.P256.Definitions
+open Hacl.Spec.ECDSAP256.Definition
 open Hacl.Spec.P256.Lemmas
 
 open Lib.ByteSequence
@@ -9,6 +9,8 @@ open Lib.IntTypes
 open Lib.Sequence
 
 
+let prime = prime_p256_order 
+let nat_prime = (n: nat {n < prime})
 
 
 let scalar = lbytes 32
@@ -17,4 +19,37 @@ let ith_bit (k:lbytes 32) (i:nat{i < 256}) : uint64 =
   let q = i / 8 in let r = size (i % 8) in
   to_u64 ((index k q >>. r) &. u8 1)
 
+let ( *% ) a b = (a * b) % prime
+
+
+val _exp_step0: p: nat_prime -> q: nat_prime -> tuple2 nat_prime nat_prime
+
+let _exp_step0 r0 r1 = 
+  let r1 = r0 *% r1 in 
+  let r0 = r0 *% r0 in 
+  r0, r1
+
+val _exp_step1: p: nat_prime -> q: nat_prime -> tuple2 nat_prime nat_prime 
+
+let _exp_step1 r0 r1 = 
+  let r0 = r0 *% r1 in 
+  let r1 = r1 *% r1 in 
+  (r0, r1)
+
+
+val _exp_step: k: scalar->  i: nat{i < 256} ->  (tuple2 nat_prime nat_prime) -> Tot (r: tuple2 nat_prime nat_prime)
+
+let _exp_step k i (p, q) = 
+  let bit = 255 - i in 
+  let bit = ith_bit k bit in 
+  let open Lib.RawIntTypes in 
+  if uint_to_nat bit = 0 then 
+      _exp_step1 p q 
+  else _exp_step0 p q  
+
+
+val exponent_spec: k: scalar -> tuple2 nat_prime nat_prime -> Tot (tuple2 nat_prime nat_prime)
+
+let exponent_spec k (p, q) = 
+  Lib.LoopCombinators.repeati 256  (_exp_step k) (p, q)
 
